lectures/lecture4/BinSearch.dfy
@@ -1,8 +1,39 @@
+// Define a predicate - "what an array being sorted is"
+predicate sorted(a: array<int>)
+  reads a
+{
+  forall j, k :: 0 <= j < k < a.Length ==> a[j] <= a[k]
+}
+
+lemma Foo (a: array<int>, low : int, high: int, value: int) 
+    requires 0 <= a.Length && sorted(a)
+    requires 0 <= low <= high <= a.Length
+    requires forall i :: 0 <= i < a.Length && !(low <= i < high) ==> a[i] != value
+    
+    ensures forall j :: 0 <= j < low ==> a[j] != value
+    ensures forall j :: high < j < a.Length ==> a[j] != value
+    {
+    
+    }
+
 // Binary Search Method
 method BinarySearch(a: array<int>, value: int) returns (index: int)
+  // Precondition:
+  // When a is a sorted array with non-negative length...
+  requires 0 <= a.Length && sorted(a)
+  // Postconditions:
+  // ...then the result (index) is either:
+  // 1. non-negative, in which case it points to "value" in a
+  ensures 0 <= index ==> index < a.Length && a[index] == value
+  // 2. negative, in which case the value doesn't exist
+  ensures index < 0 ==> forall k :: 0 <= k < a.Length ==> a[k] != value
 {
   var low, high := 0, a.Length;
   while low < high
+    invariant 0 <= low <= high <= a.Length
+    //invariant forall j :: 0 <= j < low ==> a[j] != value
+    //invariant forall j :: high < j < a.Length ==> a[j] != value
+    invariant forall i :: 0 <= i < a.Length && !(low <= i < high) ==> a[i] != value
   {
     var mid := (low + high) / 2;
     if a[mid] < value {
@@ -15,3 +46,18 @@ method BinarySearch(a: array<int>, value: int) returns (index: int)
   }
   return -1;
 }
+
+
+
+
+
+
+
+
+
+
+
+
+    // Invariants are required to prove facts about loops
+  //  invariant 0 <= low <= high <= a.Length
+    //invariant forall i :: 0 <= i < a.Length && !(low <= i < high) ==> a[i] != value
