lectures/lecture4/findMinVal.dfy
@@ -1,0 +1,16 @@
+method FindMinVal (a : array<int>) returns (min : int)
+    requires a.Length > 0  // Precondition
+    ensures forall i : int :: 0 <= i < a.Length ==> min <= a[i] // Postcondition
+{
+  min := a[0];
+  var i:= 1;
+  while (i < a.Length)
+    invariant i <= a.Length
+    invariant forall j :: 0 <= j < i ==> min <= a[j]
+  {
+    if a[i] < min
+      { min := a[i]; }
+    i := i+1;
+  }
+  assert (forall j :: 0 <= j < a.Length ==> min <= a[j]);
+}
