lectures/lecture5/HoareLogicAssertions.dfy
@@ -1,0 +1,1240 @@
+/** Hoare Triples and Dafny */
+
+/** A _Hoare triple_ is a claim about the state before and
+    after executing a statement.  The standard notation is
+
+      {P} s {Q}
+
+    meaning:
+
+      - If statement s begins execution in a state satisfying assertion P,
+      - and if s eventually terminates in some final state,
+      - then that final state will satisfy the assertion Q.
+
+    Assertion P is called the _precondition_ of the triple, and Q is
+    the _postcondition_.
+
+    For example,
+
+    - {x == 0} x := x + 1 {x == 1} is a valid Hoare triple,
+      stating that the statement x := x + 1 would transform a state in
+      which x == 0 to a state in which x == 1.
+
+    - forall m, {x == m} x := x + 1 {x == m + 1}, is a
+      _proposition_ stating that the Hoare triple {x == m} x := x +
+      m {x == m + 1} is valid for any choice of m.  Note that m
+      in the two assertions and the command in the middle is a
+      reference to the _Dafny_ variable m, which is bound outside the
+      Hoare triple. */
+
+/* ################################################################# */
+/** * Proof Rules 
+
+    The goal of Hoare logic is to provide a _compositional_
+    method for proving the validity of specific Hoare triples.  That
+    is, we want the structure of a program's correctness proof to
+    mirror the structure of the program itself.  To this end, in the
+    sections below, we'll introduce a rule for reasoning about each of
+    the different syntactic forms of statements in Dafny -- one for
+    assignment, one for sequencing, one for conditionals, etc. -- plus
+    a couple of "structural" rules for gluing things together.  We
+    will then be able to prove programs correct using these proof
+    rules. */
+
+/* ================================================================= */
+/** ** Empty statement blocks 
+
+    Since empty statement blocks don't change the state, they preserve any
+    assertion [P]:
+
+      ---------------------  (hoare_skip)
+         { P } {} { P }
+*/
+
+/* ================================================================= */
+/** ** Sequencing 
+
+    If statement s1 takes any state where P holds to a state where
+    Q holds, and if s2 takes any state where Q holds to one
+    where R holds, then doing s1 followed by s2 will take any
+    state where P holds to one where R holds:
+
+           { P } s1 { Q }
+           { Q } s2 { R }
+       ----------------------  (hoare_seq)
+         { P } s1; s2 { R }
+*/
+
+/* ================================================================= */
+/** ** Assignment 
+
+    The rule for assignment is the most fundamental of the Hoare
+    logic proof rules.  Here's how it works.
+
+    Consider this incomplete Hoare triple:
+
+       { ??? }  x := y  { x == 1 }
+
+    We want to assign y to x and finish in a state where x is 1.
+    What could the precondition be?
+
+    One possibility is y == 1, because if y is already 1 then
+    assigning it to x causes x to be 1.  That leads to a valid
+    Hoare triple:
+
+       { y == 1 }  x := y  { x == 1 }
+
+    It may seem as though coming up with that precondition must have
+    taken some clever thought.  But there is a mechanical way we could
+    have done it: if we take the postcondition x == 1 and in it
+    replace x with y---that is, replace the left-hand side of the
+    assignment statement with the right-hand side---we get the
+    precondition, y = 1. 
+
+    That same idea works in more complicated cases.  For
+    example:
+
+       { ??? }  x := x + y  { x == 1 }
+
+    If we replace the x in x == 1 with x + y, we get x + y == 1.
+    That again leads to a valid Hoare triple:
+
+       { x + y == 1 }  x := x + y  { x == 1 }
+
+    Why does this technique work?  The postcondition identifies some
+    property P that we want to hold of the variable x being
+    assigned.  In this case, P is "equals 1".  To complete the
+    triple and make it valid, we need to identify a precondition that
+    guarantees that property will hold of x.  Such a precondition
+    must ensure that the same property holds of _whatever is being
+    assigned to_ x.  So, in the example, we need "equals 1" to
+    hold of x + y.  That's exactly what the technique guarantees. 
+
+    In general, the postcondition could be some arbitrary assertion
+    Q, and the right-hand side of the assignment could be some
+    arbitrary arithmetic expression a:
+
+       { ??? }  x := a  { Q }
+
+    The precondition would then be Q, but with any occurrences of
+    x in it replaced by a.
+
+    Let's introduce a notation for this idea of replacing occurrences:
+    Define Q[x := a] to mean "Q where a is substituted in
+    place of x".
+
+    This yields the Hoare logic rule for assignment:
+
+      ---------------------------- (hoare_asgn)
+      { Q[x := a] }  x := a  { Q }
+
+    One way of reading this rule is: If you want statement x := a
+    to terminate in a state that satisfies assertion Q, then it
+    suffices to start in a state that also satisfies Q, except
+    where a is substituted for every occurrence of x. *)
+
+    To many people, this rule seems "backwards" at first, because
+    it proceeds from the postcondition to the precondition.  Actually
+    it makes good sense to go in this direction: the postcondition is
+    often what is more important, because it characterizes what we
+    can assume afer running the code.
+
+    Nonetheless, it's also possible to formulate a "forward" assignment
+    rule. 
+*/
+
+/** Here are some valid instances of the assignment rule:
+
+      { (x <= 5) [x := x + 1] }   (that is, x + 1 <= 5)
+        x := x + 1
+      { x <= 5 }
+
+      { (x == 3) [x := 3] }        (that is, 3 = 3)
+        x := 3
+      { x = 3 }
+
+      { (0 <= x && x <= 5) [x := 3]  (that is, 0 <= 3 && 3 <= 5)
+        x := 3
+      { 0 <= x && x <= 5 }
+*/
+
+/* ================================================================= */
+/** ** Consequence 
+
+    Sometimes the preconditions and postconditions we get from the
+    Hoare rules won't quite be the ones we want in the particular
+    situation at hand -- they may be logically equivalent but have a
+    different syntactic form that fails to unify with the goal we are
+    trying to prove, or they actually may be logically weaker (for
+    preconditions) or stronger (for postconditions) than what we need. 
+
+    For instance,
+
+      {(x == 3) [x := 3]} x := 3 {x == 3},
+
+    follows directly from the assignment rule, but
+
+      {true} x := 3 {x == 3}
+
+    does not.  This triple is valid, but it is not an instance of
+    [hoare_asgn] because true and (x == 3) [x := 3] are not
+    syntactically equal assertions.
+
+    However, they are logically _equivalent_, so if one triple is
+    valid, then the other must certainly be as well.  We can capture
+    this observation with the following rule:
+
+                {P'} s {Q}
+                  P <-> P'
+         -------------------------   (hoare_consequence_pre_equiv)
+                 {P} s {Q}
+
+
+    Taking this line of thought a bit further, we can see that
+    strengthening the precondition or weakening the postcondition of a
+    valid triple always produces another valid triple. This
+    observation is captured by two _Rules of Consequence_.
+
+                {P'} c {Q}
+                  P -> P'
+         -----------------------------   (hoare_consequence_pre)
+                {P} s {Q}
+
+                {P} s {Q'}
+                 Q' -> Q
+         -----------------------------    (hoare_consequence_post)
+                {P} s {Q}
+*/
+
+/* ================================================================= */
+/** ** Conditionals 
+
+    What sort of rule do we want for reasoning about conditional
+    statements?
+
+    Certainly, if the same assertion Q holds after executing
+    either of the branches, then it holds after the whole conditional.
+    So we might be tempted to write:
+
+              {P} s1 {Q}
+              {P} s2 {Q}
+      ---------------------------------
+       {P} if b { s1 } else { s2 } {Q}
+
+    However, this is rather weak. For example, using this rule,
+    we cannot show
+   
+      { true }
+        if x <= 0
+          { y := 2 }
+        else 
+          { y := x + 1 }
+      { x <= y }
+   
+    since the rule tells us nothing about the state in which the
+    assignments take place in the "then" and "else" branches.
+
+    Fortunately, we can say something more precise.  In the
+    "then" branch, we know that the boolean expression b evaluates to
+    true, and in the "else" branch, we know it evaluates to false.
+    Making this information available in the premises of the rule gives
+    us more information to work with when reasoning about the behavior
+    of s1 and s2 (i.e., the reasons why they establish the
+    postcondition Q).
+
+                {P &&  b} s1 {Q}
+                {P && !b} s2 {Q}
+      -------------------------------------  (hoare_if)
+         {P} if b { s1 } else { s2 } {Q}
+*/
+
+/*
+    {true}
+      if (x < 0)
+        { 
+          y := -x;
+        }
+      else 
+        {
+          x := x;
+        }
+    {y >= 0}
+
+    {P &&  b} s1 {Q} -> {true && x < 0} y := -x; {y > 0}
+                        {true && x < 0} -> {-x > 0}
+                                              y := -x;
+                                            { y >= 0 }
+    {P && !b} s2 {Q} -> {true && !(x < 0) x := -x; { y > 0}}
+*/
+
+/* ================================================================= */
+/** ** While Loops 
+
+    The Hoare rule for while loops is based on the idea of an
+    _invariant_: an assertion whose truth is guaranteed before and
+    after executing a statement.  An assertion P is an invariant of s if
+
+      {P} s {P}
+
+    holds.  Note that in the middle of executing s, the invariant
+    might temporarily become false, but by the end of s, it must be
+    restored. 
+
+    As a first attempt at a [while] rule, we could try:
+
+            {P} s {P}
+      ---------------------
+      {P} while b { s } {P}
+
+    That rule is valid: if P is an invariant of s, as the premise
+    requires, then no matter how many times the loop body executes,
+    s is going to be true when the loop finally finishes.
+
+    But the rule also omits two crucial pieces of information.  First,
+    the loop terminates when b becomes false.  So we can strengthen
+    the postcondition in the conclusion:
+
+              {P} s {P}
+      ---------------------------
+      {P} while b { s } {P && !b}
+
+    Second, the loop body will be executed only if [b] is true.  So we
+    can also strengthen the precondition in the premise:
+
+            {P && b} s {P}
+      --------------------------- (hoare_while)
+      {P} while b { s } {P && !b}
+
+    That is the Hoare [while] rule.  Note how it combines
+    aspects of empty blocks and conditionals:
+
+    - If the loop body executes zero times, the rule is like an empty block in
+      that the precondition survives to become (part of) the postcondition.
+
+    - Like a conditional, we can assume guard b holds on entry to
+      the substatement
+*/
+
+/* ################################################################# */
+/** * Decorated Programs */
+
+/** The beauty of Hoare Logic is that it is _structure-guided_: the
+    structure of proofs exactly follows the structure of programs.
+
+    We can record the essential ideas of a Hoare-logic proof --
+    omitting low-level calculational details -- by "decorating" a
+    program with appropriate assertions on each of its commands.
+
+    Such a _decorated program_ carries within itself an argument for
+    its own correctness. 
+
+    For example, consider the program: 
+ */
+method LoopToZero_1(m : int, p : int) returns (x: int, z: int) {
+  x := m;
+  z := p;
+  while x > 0 {
+    z := z - 1;
+    x := x - 1;
+  }
+}
+
+/* 
+    Here is one possible specification for this program, in the
+    form of a Hoare triple:
+
+    { true }
+    x := m;
+    z := p;
+    while x > 0 {
+      z := z - 1;
+      x := x - 1;
+    }
+    { z == p - m }
+
+    and here is the equivalent specification in terms of 
+    Dafny's _requires_ and _ensures_ syntax (of course,
+    Dafny can't prove this without an invariant annotation):
+*/
+method LoopToZero_2(m : nat, p : int) returns (x: nat, z: int)
+  requires true
+  ensures z == p - m
+{
+  x := m;
+  z := p;
+  while x > 0 
+    invariant (z - x == p - m)
+  {
+    z := z - 1;
+    x := x - 1;
+  }
+}
+
+/*
+//  Here is a decorated version of this program, embodying a
+//  proof of this specification:
+{
+    // { true } ->
+    // { m == m }
+      x := m;
+    // { x == m } ->
+    // { x == m && p == p };
+      z := p;
+    // { x == m && z == p } ->
+    // { z - x == p - m }
+      while x > 0 {
+        // { z - x == p - m && x > 0 } ->
+        // { (z - 1) - (x - 1) == p - m }
+        z := z - 1
+        // { z - (x - 1) == p - m };
+        x := x - 1
+        // { z - x == p - m } 
+      }
+    // { z - x == p - m && !(x > 0) } ->
+    // { z == p - m }
+}
+*/
+
+/** That is, a decorated program consists of the program's text
+    interleaved with assertions (sometimes multiple assertions
+    separated by implications). 
+
+    A decorated program can be viewed as a compact representation of a
+    proof in Hoare Logic: the assertions surrounding each command
+    specify the Hoare triple to be proved for that part of the program
+    using one of the Hoare Logic rules, and the structure of the
+    program itself shows how to assemble all these individual steps
+    into a proof for the whole program. 
+
+    Dafny's goal is to verify such decorated programs "mostly
+    automatically."  But, before we can verify anything, we need to be
+    able to _find_ a proof for a given specification, and for this we
+    need to discover the right assertions. This can be done in an
+    almost mechanical way, with the exception of finding loop
+    invariants. We'll first explain in detail how to construct 
+    decorations for several short programs, all of which are 
+    loop-free or have simple loop invariants. We'll return
+    to finding more interesting loop invariants later. 
+*/
+
+/* ================================================================= */
+/** ** Example: Swapping 
+
+    Consider the following program, which swaps the values of two
+    variables using addition and subtraction (instead of by assigning
+    to a temporary variable).
+
+       x := x + y;
+       y := x - y;
+       x := x - y
+
+    We can give a proof, in the form of decorations, that this program is
+    correct -- i.e., it really swaps x and y -- as follows.
+
+    (1)    { x == m && y == n } -> PRECONDITION #1
+    (2)    { (x + y) - ((x + y) - y) == n && (x + y) - y == m } SUB (x + y) FOR x FROM (3) #5
+             x := x + y;
+    (3)    { x - (x - y) == n && x - y == m } SUBSTITUTE (x - y) FOR y FROM (4) #4
+             y := x - y;
+    (4)    { x - y == n && y = m } SUBSTITUTE x - y FOR THE ASSIGNMENT OF x FROM (5) #3
+             x := x - y
+    (5)    { x = n && y = m } POSTCONDITION #2
+
+    The decorations can be constructed as follows:
+
+      - We begin with the undecorated program (the unnumbered lines).
+
+      - We add the specification -- i.e., the outer precondition (1)
+        and postcondition (5). In the precondition, we use parameters
+        m and n to remember the initial values of variables x
+        and y so that we can refer to them in the postcondition (5).
+
+      - We work backwards, mechanically, starting from (5) and
+        proceeding until we get to (2). At each step, we obtain the
+        precondition of the assignment from its postcondition by
+        substituting the assigned variable with the right-hand-side of
+        the assignment. For instance, we obtain (4) by substituting
+        x with x - y in (5), and we obtain (3) by substituting y
+        with x - y in (4).
+
+    Finally, we verify that (1) logically implies (2) -- i.e., that
+    the step from (1) to (2) is a valid use of the law of
+    consequence -- by doing a bit of high-school algebra.
+*/
+
+/* ================================================================= */
+/** ** Example: Simple Conditionals 
+
+    Here is a simple decorated program using conditionals,
+    assuming x, y, and z are natural numbers (as in: non-negative 
+    integers):
+
+      (1)   { true }
+              if x <= y {
+      (2)      { true && x <= y } ->
+      (3)      { (y - x) + x == y || (y - x) + y == x }
+                 z := y - x
+      (4)      { z + x == y || z + y == x }
+              } else {
+      (5)       { true && ~(x <= y) } ->
+      (6)       { (x - y) + x == y || (x - y) + y = x }
+                z := x - y
+      (7)       { z + x = y || z + y = x }
+              }
+      (8)   { z + x = y || z + y = x }
+
+/* from class:
+  {true}
+  if x <= y {
+    {true && x <= y} ->
+    {(y - x) + x == y || (y - x) + y == x}
+    z := y - x;
+  } else {
+    { true && ~(x <= y) } ->
+    {(x - y) + x == y || (x - y) + y == x}
+    z := x - y;
+  }
+  {z + x == y || z + y == x}
+
+*/
+
+These decorations can be constructed as follows:
+
+  - We start with the outer precondition (1) and postcondition (8).
+
+  - Following the format dictated by the [hoare_if] rule, we copy the
+    postcondition (8) to (4) and (7). We conjoin the precondition (1)
+    with the guard of the conditional to obtain (2). We conjoin (1)
+    with the negated guard of the conditional to obtain (5).
+
+  - In order to use the assignment rule and obtain (3), we substitute
+    z by y - x in (4). To obtain (6) we substitute z by x - y
+    in (7).
+
+  - Finally, we verify that (2) implies (3) and (5) implies (6). Both
+    of these implications crucially depend on the ordering of x and
+    y obtained from the guard. For instance, knowing that x <= y
+    ensures that subtracting x from y and then adding back x
+    produces y, as required by the first disjunct of (3). Similarly,
+    knowing that !(x <= y)] ensures that subtracting y from x
+    and then adding back y produces x, as needed by the second
+    disjunct of (6). Note that n - m + m = n does _not_ hold for
+    arbitrary natural numbers n and m (Dafny, in particular, won't
+    even let you perform a subtraction that would get you in the 
+    negatives)
+*/
+/*
+method nat_test(m: nat, n : nat) returns (x : nat, y : nat) 
+  ensures (x == y)
+{
+  x := m - n;
+  y := n - m; 
+}
+*/
+
+/* ================================================================= */
+/** ** Example: Reduce to Zero 
+
+    Here is a while loop that is so simple that true suffices
+    as a loop invariant when x is a nat:
+
+        (1)    {true}
+                 while x > 0 {
+        (2)       { true && x > 0 } ->
+        (3)       { true }
+                   x := x - 1
+        (4)       { true }
+                 }
+        (5)    { true && !(x > 0) } -> HOARE_WHILE
+        (6)    { x = 0 }
+
+   The decorations can be constructed as follows:
+
+     - Start with the outer precondition (1) and postcondition (6).
+
+     - Following the format dictated by the [hoare_while] rule, we copy
+       (1) to (4). We conjoin (1) with the guard to obtain (2). We also
+       conjoin (1) with the negation of the guard to obtain (5).
+
+     - Because the final postcondition (6) does not syntactically match (5),
+       we add an implication between them.
+
+     - Using the assignment rule with assertion (4), we trivially substitute
+       and obtain assertion (3).
+
+     - We add the implication between (2) and (3).
+
+   Finally we check that the implications do hold; both are trivial. */
+
+
+/* ================================================================= */
+/** ** Example: Division 
+
+    Let's do one more example of simple reasoning about a loop.
+
+    The following program calculates the integer quotient and
+    remainder of parameters m and n. 
+    (Dafny complains about the invariant and the loop's termination. 
+    How would you fix the latter?)
+*/
+
+// method QuotDiv (m : int, n : int) returns (x : int, y : int) 
+//   requires true
+//   ensures n * y + x == m && x < n
+// {
+//        x := m;
+//        y := 0;
+//        while n <= x
+//         invariant n * y + x == m
+//        {
+//          x := x - n;
+//          y := y + 1;
+//        }
+// }
+
+/*  If we execute this program, it will terminate with the variable
+    x set to the remainder when m is divided by n and y set to the 
+    quotient. 
+
+    In order to give a specification to this program we need to
+    remember that dividing m by n produces a remainder x and a
+    quotient y such that n * y + x == m && x < n].
+
+    It turns out that we get lucky with this program and don't have to
+    think very hard about the loop invariant: the invariant is just
+    the first conjunct, [n * y + x == m] INVARIANT (NEEDS TO HOLD BEFORE WHILE LOOP), 
+    and we can use this to decorate the program.
+
+      (1)  { true } ->
+      (2)  { n * 0 + m == m }
+             x := m;
+      (3)  { n * 0 + x == m }
+             y := 0;
+      (4)  { n * y + x == m }
+             while n <= x {
+      (5)  { n * y + x == m && n <= x } ->
+      (6)  { n * (y + 1) + (x - n) == m }
+               x := x - n;
+      (7)  { n * (y + 1) + x == m }
+               y := y + 1
+      (8)  { n * y + x == m }
+             }
+      (9)  { n * y + x == m && !(n <= x) } -> 
+     (10)  { n * y + x == m && x < n }
+
+    Assertions (4), (5), (8), and (9) are derived mechanically from
+    the invariant and the loop's guard.  Assertions (8), (7), and (6)
+    are derived using the assignment rule going backwards from (8)
+    to (6).  Assertions (4), (3), and (2) are again backwards
+    applications of the assignment rule.
+
+    Now that we've decorated the program it only remains to check that
+    the uses of the consequence rule are correct -- i.e., that (1)
+    implies (2), that (5) implies (6), and that (9) implies (10). This
+    is indeed the case:
+      - (1) -> (2):  trivial, by algebra.
+      - (5) -> (6):  because [n <= x], we are guaranteed that the
+        subtraction in (6) does not get zero-truncated.  We can
+        therefore rewrite (6) as [n * y + n + x - n] and cancel the
+        ns, which results in the left conjunct of (5).
+      - (9) -> (10):  if [!(n <= x)] then [x < n].  That's straightforward
+        from high-school algebra.
+
+    So, we have a valid decorated program. 
+    */
+
+/* ################################################################# */
+/** * Finding Loop Invariants 
+
+    Once the outermost precondition and postcondition are
+    chosen, the only creative part of a verifying program using Hoare
+    Logic is finding the right loop invariants.  The reason this is
+    difficult is the same as the reason that inductive mathematical
+    proofs are:
+
+    - Strengthening a _loop invariant_ means that you have a stronger
+      assumption to work with when trying to establish the
+      postcondition of the loop body, but it also means that the loop
+      body's postcondition is stronger and thus harder to prove.
+
+    - Strengthening an _induction hypothesis_ means that you have a
+      stronger assumption to work with when trying to complete the
+      induction step of the proof, but it also means that the
+      statement being proved inductively is stronger and thus harder
+      to prove.
+
+    This section explains how to approach the challenge of finding
+    loop invariants through a series of examples and exercises. */
+
+/* ================================================================= */
+/** ** Example: Slow Subtraction 
+
+    The following program subtracts the value of x from the value of
+    y by repeatedly decrementing both x and y.  We want to verify its
+    correctness with respect to the pre- and postconditions shown:
+    
+           { x == m && y == n }
+             while !(x == 0) do
+               y := y - 1;
+               x := x - 1
+             end
+           { y = n - m }
+
+    To verify this program, we need to find an invariant [Inv] for the
+    loop.  As a first step we can leave [Inv] as an unknown and build a
+    _skeleton_ for the proof by applying the rules for local
+    consistency, working from the end of the program to the beginning,
+    as usual, and without any thinking at all yet. *)
+
+(** This leads to the following skeleton: Inv = Invariant
+
+        (1)    { x == m && y == n }  ->                   (a)
+        (2)    { Inv }
+                 while x > 0 {}
+        (3)    { Inv && x > 0 }  ->                       (c)
+        (4)    { Inv [x := x-1] [y := y-1] } from (4.5) and (5.5)
+                   y := y - 1;
+        (5)    { Inv [x := x-1] }
+                   x := x - 1
+        (6)    { Inv }
+                 }
+        (7)    { Inv && !(x > 0) }  ->                    (b)
+        (8)    { y == n - m }
+
+    By examining this skeleton, we can see that any valid [Inv] will
+    have to respect three conditions:
+    - (a) it must be _weak_ enough to be implied by the loop's
+      precondition, i.e., (1) must imply (2);
+    - (b) it must be _strong_ enough to imply the program's postcondition,
+      i.e., (7) must imply (8);
+    - (c) it must be _preserved_ by each iteration of the loop (given
+      that the loop guard evaluates to true), i.e., (3) must imply (4). 
+
+    These conditions are actually independent of the particular
+    program and specification we are considering: every loop
+    invariant has to satisfy them.
+
+    One way to find an invariant that simultaneously satisfies these
+    three conditions is by using an iterative process: start with a
+    "candidate" invariant (e.g., a guess or a heuristic choice) and
+    check the three conditions above; if any of the checks fails, try
+    to use the information that we get from the failure to produce
+    another -- hopefully better -- candidate invariant, and repeat.
+
+    For instance, in the reduce-to-zero example above, we saw that,
+    for a very simple loop, choosing [true] as an invariant did the
+    job.  Maybe it will work here too.  To find out, let's try
+    instantiating [Inv] with [true] in the skeleton above and
+    see what we get...
+
+        (1)    { x == m && y == n } ->                    (a - OK)
+        (2)    { true }
+                 while x > 0 {}
+        (3)    { true && x > 0 } ->                       (c - OK)
+        (4)    { true }
+                   y := y - 1;
+        (5)    { true }
+                   x := x - 1
+        (6)    { true }
+                 }
+        (7)    { true && !(x > 0) } ->                 (b - WRONG!)
+        (8)    { y == n - m }
+
+    While conditions (a) and (c) are trivially satisfied,
+    (b) is wrong: it is not the case that [true && !(x > 0)] (7)
+    implies [y == n - m] (8).  In fact, the two assertions are
+    completely unrelated, so it is very easy to find a counterexample
+    to the implication (say, [y = x = m = 0] and [n = 1]).
+
+    If we want (b) to hold, we need to strengthen the invariant so
+    that it implies the postcondition (8).  One simple way to do
+    this is to let the invariant _be_ the postcondition.  So let's
+    return to our skeleton, instantiate [Inv] with [y == n - m], and
+    try checking conditions (a) to (c) again.
+
+    (1)    { x == m && y == n } ->              (a - WRONG!)
+    (2)    { y == n - m }
+             while x > 0 do
+    (3)    { y == n - m && x > 0 } ->           (c - WRONG!)
+    (4)    { y - 1 == n - m }
+               y := y - 1;
+    (5)    { y == n - m }
+               x := x - 1
+    (6)    { y == n - m }
+             }
+    (7)    { y == n - m && !(x > 0) } ->            (b - OK) (x is natural number)
+    (8)    { y == n - m }
+
+    This time, condition (b) holds trivially, but (a) and (c) are
+    broken. Condition (a) requires that (1) [x == m && y == n]
+    implies (2) [y == n - m].  If we substitute y by n we have to
+    show that [n == n - m] for arbitrary m and n, which is not
+    the case (for instance, when m = n = 1).  Condition (c) requires
+    that [n - m - 1 == n - m], which fails, for instance, for n = 1
+    and m = 0. So, although [y == n - m] holds at the end of the loop,
+    it does not hold from the start, and it doesn't hold on each
+    iteration; it is not a correct invariant.
+
+    This failure is not very surprising: the variable y changes
+    during the loop, while m and n are constant, so the assertion
+    we chose didn't have much chance of being an invariant!
+
+    To do better, we need to generalize (7) to some statement that is
+    equivalent to (8) when x is 0, since this will be the case
+    when the loop terminates, and that "fills the gap" in some
+    appropriate way when x is nonzero.  Looking at how the loop
+    works, we can observe that x and y are decremented together
+    until x reaches 0.  So, if [x == 2] and [y == 5] initially,
+    after one iteration of the loop we obtain [x == 1] and [y == 4];
+    after two iterations [x == 0] and [y == 3]; and then the loop stops.
+    Notice that the difference between y and x stays constant
+    between iterations: initially, [y == n] and [x == m], and the
+    difference is always (n - m).  So let's try instantiating [Inv] in
+    the skeleton above with [y - x == n - m] INVARIANT.
+
+    (1)    { x == m && y == n } ->                            (a - OK)
+    (2)    { y - x == n - m }
+             while x > 0 {
+    (3)    { y - x == n - m && x > 0 } ->                     (c - OK)
+    (4)    { (y - 1) - (x - 1) == n - m }
+               y := y - 1;
+    (5)    { y - (x - 1) = n - m }
+               x := x - 1
+    (6)    { y - x == n - m }
+             }
+    (7)    { y - x == n - m && !(x > 0) } ->                (b - OK?)
+    (8)    { y = n - m }
+
+    Success? If everything is a natural number conditions (a), (b) 
+    and (c) all hold now; However, the same is not true if everything 
+    is an integer, as !(x > 0) does not imply x = 0! In that case, we would
+    need to further strengthen the invariant to include that x >= 0 
+    (assuming that's the case to begin with): 
+    
+    (1)    { m >= 0 && n >= 0 && x == m && y == n } ->                 (a - OK)
+    (2)    { y - x == n - m }
+             while x > 0 {
+    (3)    { x >= 0 && y - x == n - m && x > 0 } ->                    (c - OK)
+    (4)    { (x - 1) >= 0 && (y - 1) - (x - 1) == n - m }
+               y := y - 1;
+    (5)    { (x - 1) >= 0 && y - (x - 1) = n - m }
+               x := x - 1
+    (6)    { x >= 0 && y - x == n - m }
+             }
+    (7)    { x >= 0 && y - x == n - m && !(x > 0) } ->                (b - OK)
+    (8)    { y = n - m }
+*/
+
+/* ================================================================= */
+/** ** Exercise: Slow Assignment 
+
+    A roundabout way of assigning a number currently stored in x to
+    the variable y is to start y at 0, then decrement x until
+    it hits 0, incrementing y at each step. Here is a program that
+    implements this idea.  Fill in decorations and prove the decorated
+    program correct. (The proof should be very simple.) *)
+
+   { x == m }
+      y := 0
+                    { Inv [y := 0] } ->
+                    { Inv } 
+      while x > 0 {
+                    { Inv && x > 0 } ->
+                    { Inv [y := y + 1][x : x - 1] }
+         x := x - 1
+                    { Inv [y := y + 1] } ;
+         y := y + 1
+                    { Inv }
+      }
+    { Inv && !(x > 0) } ->
+    { y == m }
+
+
+START
+    { x == m } -> { Inv [y := 0] }
+    { Inv && x > 0 } -> { (x-1) + (y+1) == m }
+    { Inv && !(x > 0) } -> { y == m }
+
+#1 Inv : = x + y == m
+    { x == m } -> { x + 0 == m }
+    { x + y == m && x > 0 } -> { [y := y + 1][x : x - 1] }
+    { Inv && !(x > 0) } -> { y == m }
+
+#2 Inv : = x + y == m && x >= 0
+    { x == m } -> { x + 0 == m && x >= 0 }
+    { x + y == m && x >= 0 && x > 0 } -> { [y := y + 1][x : x - 1] } // get updated from online
+    { Inv && !(x > 0) } -> { y == m }
+*/
+
+/* ================================================================= */
+/** ** Example: Parity 
+
+    Here is a cute way of computing the parity of a value initially
+    stored in x, due to Daniel Cristofani.
+
+       { x == m }
+         while 2 <= x do
+           x := x - 2
+         end
+       { x = parity m }
+
+    The parity function used in the specification is defined in
+    as follows: 
+**/
+/*
+function parity(x:nat) : nat {
+  match x 
+  case 0 => 0
+  case 1 => 1
+  case _ => parity (x - 2)
+}
+
+method compute_partiy(M:nat) returns (x:nat) 
+  requires true
+  ensures (x == parity(m))
+{
+  // { true } ->
+  // parity(x) == parity(m)
+  x := m
+  // { partiy(x) == partiy(m) }
+  while 2 <= x 
+    invariant (partiy(x) == partiy(m)) // { P }
+  {
+    // {parity(x) == parity(m) && 2 <= x} ->
+    // {parity(x) == parity(m)}
+    x := x- 2
+    // { partiy(x) == partiy(m) }
+  }
+// { parity(x) == parity(m) && !(2 <= x)}
+// { x == parity(m) }
+} 
+*/
+
+/** The postcondition does not hold at the beginning of the loop,
+    since [m == parity m] does not hold for an arbitrary m, so we
+    cannot hope to use that as an invariant.  To find an invariant that works,
+    let's think a bit about what this loop does.  On each iteration it
+    decrements x by 2, which preserves the parity of x.  So the
+    parity of x does not change, i.e., it is invariant.  The initial
+    value of x is m, so the parity of x is always equal to the
+    parity of m. Using [parity x == parity m] as an invariant we
+    obtain the following decorated program:
+
+      { x == m } ->                                         (a - OK)
+      { parity x == parity m }
+        while 2 <= x do
+                     { parity x == parity m && 2 <= x } ->>  (c - OK)
+                     { parity (x-2) == parity m }
+          x := x - 2
+                     { parity x == parity m }
+        end
+      { parity x == parity m && !(2 <= x) } ->>              (b - OK)
+      { x = parity m }
+
+    With this invariant, conditions (a), (b), and (c) are all
+    satisfied. For verifying (b), we observe that, when [x < 2], we
+    have [parity x = x] (we can easily see this in the definition of
+    [parity]).  For verifying (c), we observe that, when [2 <= x], we
+    have [parity x = parity (x-2)]. 
+*/
+
+/* ================================================================= */
+/** ** Example: Finding Square Roots 
+
+    The following program computes the integer square root of x
+    by naive iteration:
+
+    { x == m }
+      z := 0;
+      while (z+1)*(z+1) <= x {
+        z := z+1
+      }
+    { z*z<=m && m<(z+1)*(z+1) }
+
+
+    As we did before, we can try to use the postcondition as a
+    candidate invariant, obtaining the following decorated program:
+
+    (1)  { x==m } ->                   (a - second conjunct of (2) WRONG!)
+    (2)  { 0*0 <= m && m<(0+1)*(0+1) }
+            z := 0
+    (3)  { z*z <= m && m<(z+1)*(z+1) };
+            while (z+1)*(z+1) <= x {
+    (4)  { z*z<=m && m<(z+1)*(z+1) && (z+1)*(z+1)<=x } ->>            (c - WRONG!)
+    (5)  { (z+1)*(z+1)<=m && m<((z+1)+1)*((z+1)+1) }
+              z := z+1
+    (6)  { z*z<=m && m<(z+1)*(z+1) }
+            }
+    (7)  { z*z<=m && m<(z+1)*(z+1) && !((z+1)*(z+1)<=x) } ->>  (b - OK)
+    (8)  { z*z<=m && m<(z+1)*(z+1) }
+
+    This didn't work very well: conditions (a) and (c) both failed.
+    Looking at condition (c), we see that the second conjunct of (4)
+    is almost the same as the first conjunct of (5), except that (4)
+    mentions x while (5) mentions m. But note that x is never
+    assigned in this program, so we should always have x=m. We
+    didn't propagate this information from (1) into the loop
+    invariant, but we could!
+
+    Also, we don't need the second conjunct of (8), since we can
+    obtain it from the negation of the guard -- the third conjunct
+    in (7) -- again under the assumption that [x==m].  This allows
+    us to simplify a bit.
+
+    So we now try [x==m && z*z <= m] as the loop invariant:
+
+    { x==m } ->                                           (a - OK)
+    { x==m && 0*0 <= m }
+      z := 0
+                 { x==m && z*z <= m };
+      while (z+1)*(z+1) <= x do
+                 { x==m && z*z<=m && (z+1)*(z+1)<=x } ->  (c - OK)
+                 { x==m && (z+1)*(z+1)<=m }
+        z := z + 1
+                 { x==m && z*z<=m }
+      end
+    { x=m && z*z<=m && ~((z+1)*(z+1)<=x) } ->             (b - OK)
+    { z*z<=m && m<(z+1)*(z+1) }
+
+    This works, since conditions (a), (b), and (c) are now all
+    trivially satisfied.
+
+    Very often, when a variable is used in a loop in a read-only
+    fashion (i.e., it is referred to by the program or by the
+    specification and it is not changed by the loop), it is necessary
+    to record the fact that it doesn't change in the loop invariant. */
+
+/* ================================================================= */
+method foo ()
+/** ** Example: Squaring 
+
+  Here is a program that squares [x] by repeated addition:
+
+  { x == m }
+    y := 0;
+    z := 0;
+    while y != x {
+      z := z + x;
+      y := y + 1
+    }
+  { z == m*m }
+*)
+
+(** The first thing to note is that the loop reads x but doesn't
+    change its value. As we saw in the previous example, it can be a good idea
+    in such cases to add x == m to the invariant.  The other thing
+    that we know is often useful in the invariant is the postcondition,
+    so let's add that too, leading to the candidate invariant
+    [z == m * m && x == m].
+
+    { x == m } ->                                       (a - WRONG)
+    { 0 == m*m && x == m }
+      y := 0
+    { 0 == m*m && x == m };
+      z := 0
+    { z == m*m && x == m };
+      while y != x {
+    { z == m*m && x == m && y != x } ->                (c - WRONG)
+    { z+x == m*m && x == m }
+        z := z + x
+    { z == m*m && x = m };
+        y := y + 1
+    { z == m*m && x == m }
+      }
+    { z == m*m && x == m && !(y != x) } ->>               (b - OK)
+    { z == m*m }
+
+    Conditions (a) and (c) fail because of the [z = m*m] part.  While
+    [z] starts at [0] and works itself up to [m*m], we can't expect
+    [z] to be [m*m] from the start.  If we look at how [z] progresses
+    in the loop, after the 1st iteration [z = m], after the 2nd
+    iteration [z = 2*m], and at the end [z = m*m].  Since the variable
+    [y] tracks how many times we go through the loop, this leads us to
+    derive a new invariant candidate: [z == y*m && x == m].
+
+    { x == m } ->                                       (a - OK)
+    { 0 == 0*m && x == m }
+      y := 0
+    { 0 == y*m && x == m };
+      z := 0
+    { z == y*m && x == m };
+      while y != x {
+    { z == y*m && x == m && y != x } ->                (c - OK)
+    { z+x == (y+1)*m && x == m }
+        z := z + x
+    { z == (y+1)*m && x = m };
+        y := y + 1
+    { z == y*m && x == m }
+      }
+    { z == y*m && x == m && !(y != x) } ->>               (b - OK)
+    { z == m*m }
+
+    This new invariant makes the proof go through: all three
+    conditions are easy to check.
+
+    It is worth comparing the postcondition [z == m*m] and the [z == y*m] 
+    conjunct of the invariant. It is often the case that one has
+    to replace parameters with variables -- or with expressions
+    involving both variables and parameters, like [m - y] -- when
+    going from postconditions to invariants. 
+*/
+
+/* ================================================================= */
+/** ** Exercise: Factorial 
+
+    Recall that n! denotes the factorial of n (i.e., n! =
+    1*2*...*n).  We can easily define it in Dafny as follows:
+*/
+function fact (n : nat) : nat {
+  match n 
+  case 0 => 1
+  case _ => n * (fact(n-1))
+}
+
+/* First, write the imperative Dafny program [factorial] that calculates the factorial
+   of the number initially stored in the variable x and puts it in
+   the variable y.
+*/
+
+method factorial(n:nat) returns (x:nat) 
+  requires true
+  ensures (x == fact(n))
+{
+  var i := n;
+  x := 1;
+  // fact(i) * x == fact(n)
+  while (i > 0)
+    invariant (fact(i) * x == fact(n))
+  {
+    x := x * i;
+    i := i - 1;
+  }
+}
+
+/** Using your definition [factorial], write a decorated program that
+    implements the factorial function. */
+
+/* ================================================================= */
+/** ** Exercise: Minimum 
+
+    { true } ->
+    { FILL_IN_HERE }
+      x := a
+             { FILL_IN_HERE };
+      y := b
+             { FILL_IN_HERE };
+      z := 0
+             { FILL_IN_HERE };
+      while x != 0 && y != 0 {
+             { FILL_IN_HERE } ->
+             { FILL_IN_HERE }
+        x := x - 1
+             { FILL_IN_HERE };
+        y := y - 1
+             { FILL_IN_HERE };
+        z := z + 1
+             { FILL_IN_HERE }
+      }
+    { FILL_IN_HERE } ->
+    { z == min a b }
+*/
+
+/* ================================================================= */
+/** ** Exercise: Two Loops 
+
+    Here is a pretty inefficient way of adding 3 numbers:
+
+     x := 0;
+     y := 0;
+     z := c;
+     while x != a {
+       x := x + 1;
+       z := z + 1
+     };
+     while y <> b {
+       y := y + 1;
+       z := z + 1
+     }
+
+    Show that it does what it should by completing the
+    following decorated program.
+
+Definition two_loops_dec (a b c : nat) : decorated :=
+  <{
+    { true } ->>
+    { FILL_IN_HERE }
+      x := 0
+                   { FILL_IN_HERE };
+      y := 0
+                   { FILL_IN_HERE };
+      z := c
+                   { P };
+      while x != a {
+                   { FILL_IN_HERE } ->>
+                   { FILL_IN_HERE }
+        x := x + 1
+                   { FILL_IN_HERE };
+        z := z + 1
+                   { FILL_IN_HERE }
+      end
+                   { FILL_IN_HERE } ->>
+                   { FILL_IN_HERE };
+      while y != b {
+                   { FILL_IN_HERE } ->>
+                   { FILL_IN_HERE }
+        y := y + 1
+                   { FILL_IN_HERE };
+        z := z + 1
+                   { FILL_IN_HERE }
+      }
+    { FILL_IN_HERE } ->>
+    { z == a + b + c }
+*/
+
+/* ================================================================= */
+/** ** Exercise: Power Series 
+
+    Here is a program that computes the series:
+    [1 + 2 + 2^2 + ... + 2^m = 2^(m+1) - 1]
+
+    x := 0;
+    y := 1;
+    z := 1;
+    while x != m {
+      z := 2 * z;
+      y := y + z;
+      x := x + 1;
+    }
+    end
+
+    Turn this into a decorated program and prove it correct. 
+*/
+
+function pow2(n : nat) : nat {
+  match n 
+  case 0 => 1
+  case _ => 2 * (pow2 (n-1))
+}
+
+/* 
+    { true } ->
+    { FILL_IN_HERE }
+      x := 0
+               { FILL_IN_HERE };
+      y := 1
+               { FILL_IN_HERE };
+      z := 1
+               { FILL_IN_HERE };
+      while x != n {
+               { FILL_IN_HERE } ->
+               { FILL_IN_HERE }
+        z := 2 * z
+               { FILL_IN_HERE };
+        y := y + z
+               { FILL_IN_HERE };
+        x := x + 1
+               { FILL_IN_HERE }
+      }
+    { FILL_IN_HERE } ->
+    { y == pow2 (n+1) - 1 }
+*/
