lectures/lecture7/intro-template/README.md
@@ -1,0 +1,2 @@
+Code to accompany first lectures & in-class exercises for CMSC 488X.
+Look at the course website for more details.
